src/core/Ty.v
@@ -11,12 +11,12 @@ Record tvsymbol := {
 Definition tvsymbol_eqb (t1 t2: tvsymbol) : bool :=
   ident_eqb t1.(tv_name) t2.(tv_name).
 
-Lemma tvsymbol_eqb_eq (t1 t2: tvsymbol): t1 = t2 <-> tvsymbol_eqb t1 t2.
+Lemma tvsymbol_eqb_eq (t1 t2: tvsymbol): t1 = t2 <-> 
+  tvsymbol_eqb t1 t2.
 Proof.
   unfold tvsymbol_eqb.
   rewrite <- ident_eqb_eq.
-  destruct t1 as [t1]; destruct t2 as [t2]; simpl;
-  split; intros Heq; inversion Heq; subst; reflexivity.
+  destruct t1 as [t1]; destruct t2 as [t2]; simpl; solve_eqb_eq. 
 Qed.
 
 Definition tvsymbol_eq : base.EqDecision tvsymbol :=
@@ -87,7 +87,7 @@ Inductive type_def_c : Type :=
 with ty_c : Type :=
   | mk_ty : ty_node_c -> CoqBigInt.t -> ty_c
 with tysymbol_c : Type :=
-  | mk_ts : ident -> list tvsymbol -> type_def_c -> tysymbol_c
+  | mk_ts_c : ident -> list tvsymbol -> type_def_c -> tysymbol_c
 with ty_node_c : Type :=
   | Tyvar : tvsymbol -> ty_node_c
   | Tyapp: tysymbol_c -> list ty_c -> ty_node_c.
@@ -110,1284 +110,193 @@ Definition tag_of_ty (t: ty_c) : CoqBigInt.t :=
 
 Definition ident_of_tysym (t: tysymbol_c) : ident :=
   match t with
-  | mk_ts t _ _ => t
+  | mk_ts_c t _ _ => t
   end.
 
 Definition vars_of_tysym (t: tysymbol_c) : list tvsymbol :=
   match t with
-  | mk_ts _ t _ => t
+  | mk_ts_c _ t _ => t
   end.
 
 Definition type_def_of_tysym (t: tysymbol_c) : type_def_c :=
   match t with
-  | mk_ts _ _ t => t
+  | mk_ts_c _ _ t => t
   end.
 
-(*Test with equality on ty*)
+(*Induction principle for types (TODO move)*)
+Section TyInd.
+
+Variable (P1: ty_c -> Prop).
+Variable (P2: ty_node_c -> Prop).
+Variable (P3: tysymbol_c -> Prop).
+
+Variable (Hty: forall (t: ty_c),
+  P2 (node_of_ty t) ->
+  P1 t).
+
+Variable (Hvar: forall (v: tvsymbol), P2 (Tyvar v)).
+Variable (Happ: forall (ts: tysymbol_c) (tys: list ty_c),
+  P3 ts -> Forall P1 tys -> P2 (Tyapp ts tys)).
+
+Variable (Htysym: forall (t: tysymbol_c),
+  match (type_def_of_tysym t) with
+  | Alias_c a => P1 a
+  | _ => True
+  end -> P3 t).
+
+Fixpoint ty_c_ind (t: ty_c) : P1 t :=
+  Hty t (ty_node_c_ind (node_of_ty t))
+with ty_node_c_ind (t: ty_node_c) : P2 t :=
+  match t with
+  | Tyvar v => Hvar v
+  | Tyapp ts tys => Happ ts tys (tysymbol_c_ind ts)
+    ((fix tys_ind (l: list ty_c) : Forall P1 l :=
+      match l with
+      | h :: t => Forall_cons _ h t (ty_c_ind h) (tys_ind t)
+      | nil => Forall_nil _
+      end) tys)
+  end
+with tysymbol_c_ind (t: tysymbol_c) : P3 t :=
+  Htysym t (match type_def_of_tysym t as t' return
+              (match t' with 
+              | Alias_c a => P1 a
+              | _ => True
+              end) with
+            | Alias_c a => ty_c_ind a
+            | _ => I
+  end).
+
+Definition ty_mut_ind: 
+  (forall (t: ty_c), P1 t) /\
+  (forall (t: ty_node_c), P2 t) /\
+  (forall (t: tysymbol_c), P3 t) :=
+   conj (fun t => ty_c_ind t) 
+  (conj (fun t => ty_node_c_ind t)
+  (fun t => tysymbol_c_ind t)).
+
+End TyInd.
+
+(* Decidable Equality *)
+
 Fixpoint ty_eqb (t1 t2: ty_c) : bool :=
-  CoqBigInt.eq (tag_of_ty t1) (tag_of_ty t2) &&
+  CoqBigInt.eqb (tag_of_ty t1) (tag_of_ty t2) &&
   ty_node_eqb (node_of_ty t1) (node_of_ty t2)
 with ty_node_eqb (t1 t2: ty_node_c) : bool :=
   match t1, t2 with
   | Tyvar v1, Tyvar v2 => tvsymbol_eqb v1 v2
   | Tyapp ts1 tys1, Tyapp ts2 tys2 =>
     tysymbol_eqb ts1 ts2 &&
-    ((fix tys_eqb (l1 l2: list ty_c) : bool :=
-      match l1, l2 with
-      | h1 :: t1, h2 :: t2 => ty_eqb h1 h2 && tys_eqb t1 t2
-      | nil,nil => true
-      | _, _ => false
-      end) tys1 tys2)
+    (*TODO: not great - use OCaml length?*)
+    Nat.eqb (length tys1) (length tys2) &&
+    forallb id (map2 ty_eqb tys1 tys2)
   | _, _ => false
   end
 with tysymbol_eqb (t1 t2: tysymbol_c) : bool :=
   ident_eqb (ident_of_tysym t1) (ident_of_tysym t2) &&
   list_eqb tvsymbol_eqb (vars_of_tysym t1) (vars_of_tysym t2) &&
   match type_def_of_tysym t1, type_def_of_tysym t2 with
-  | NoDef_c, Nodef_c => true
+  | NoDef_c, NoDef_c => true
   | Alias_c a1, Alias_c a2 => ty_eqb a1 a2
   | Range_c n1, Range_c n2 => Number.int_range_eqb n1 n2
   | Float_c f1, Float_c f2 => Number.float_format_eqb f1 f2
   | _, _ => false
   end.
 
-(*Arguments ty_rec {A}.
-Arguments ty_node {A}.
-Arguments ty_tag {A}.*)
-
-
-
-(*Arguments tysymbol_ {A}.
-Arguments ts_name {A}.
-Arguments ts_args {A}.
-Arguments ts_def {A}.
-
-Inductive ty_node__ : Type :=
-  | Tyvar_ : tvsymbol -> ty_node__
-  | Tyapp_ : @tysymbol_ ty_node__ -> list (@ty_ ty_node__) -> ty_node__.
-*)
-(*Definition ty' := @ty_ ty_node__.
-
-Definition tysymbol' := @tysymbol_ ty_node__.*)
-
-
-
-
-(*Try again*)
-(*
-
-(*This is surprisingly difficult to deal with, because 
-  Coq does not support mixed Record and Inductive mutually
-  recursive types (why3 uses these extensively).
-  We want to mantain compatibility with the API, as external
-  clients like Frama-C do in fact use record notation on these
-  values. 
-  There is a way to encode this by making the recursive argument
-  polymorphic and instantiating it later with itself.
-  This results in the OCaml types we expect, at the cost of
-  being able to write Fixpoint functions, since Coq can no
-  longer tell such definitions are well-founded.
-  We can fix this by defining a size metric and doing
-  well-founded recursion (as in Well-Founded Recursion
-  Done Right). But this is painful to do for every function,
-  and generic functions (say, an induction principle)*)
-
-Inductive type_def (A: Type) : Type :=
-  | NoDef
-  | Alias: A -> type_def A
-  | Range: Number.int_range -> type_def A
-  | Float: Number.float_format -> type_def A.
-
-(*We do this to get around the restriction that
-  Coq Records and Inductives cannot be mutually recursive
-  with each other. TODO: see if we can ensure that
-  this satisfies the correct .mli file*)
-Record ty_ (A: Type) := 
-  { ty_node: A;
-    ty_tag: CoqBigInt.t}.
-
-Arguments ty_ {A}.
-Arguments ty_node {A}.
-Arguments ty_tag {A}.
-
-Record tysymbol_ (A: Type) := {
-  ts_name : ident;
-  ts_args : list tvsymbol;
-  ts_def : type_def (@ty_ A)
-}.
-
-Arguments tysymbol_ {A}.
-Arguments ts_name {A}.
-Arguments ts_args {A}.
-Arguments ts_def {A}.
-
-Inductive ty_node_ : Type :=
-  | Tyvar : tvsymbol -> ty_node_
-  | Tyapp : @tysymbol_ ty_node_ -> list (@ty_ ty_node_) -> ty_node_.
-
-Definition ty := @ty_ ty_node_.
-
-Definition tysymbol := @tysymbol_ ty_node_.
-
-(*This encoding satisfies the expected OCaml interface
-  (with a mixed record-inductive type), but because Coq
-  does not allow us to write this directly, we do not
-  have a good induction principle. While we could
-  (and TODO maybe will) prove an induction principle,
-  we instead give a simpler construction for writing
-  the kinds of functions we will need: those that
-  take a [ty] and match on the [ty_node].
-  First, we need well-foundedness, so we define a size*)
-Section TyFuncs.
-
-Section TySize.
-
-
-(*TODO: try with Xavier trick (Equations bad extraction I think) and manual rec*)
-(*Define size*)
-Fixpoint ty_node_size (t: ty_node_) : nat :=
-  match t with
-  | Tyvar v => 1
-  | Tyapp ts tys => 1 +
-    (*tysymbol size*)
-    (1 + match (ts_def ts) with
-          | NoDef _ => 0
-          | Alias _ x => 1 + (1 + ty_node_size (x.(ty_node)))
-          | _=> 1
-    end) +
-  
-   list_sum 
-      (map (fun (x: ty) => 1 + ty_node_size (x.(ty_node))) tys)
-  end.
-
-Definition ty_size (t: ty) : nat :=
-  1 + ty_node_size (t.(ty_node)).
-
-Definition tysymbol_size (ts: tysymbol) : nat :=
-  1 + match ts_def ts with
-    | NoDef _ => 0
-    | Alias _ x => 1 + ty_size x
-    | _ => 1
-  end.
-
-Lemma ty_node_size_rewrite (t: ty_node_) :
-  ty_node_size t =
-  match t with
-  | Tyvar v => 1
-  | Tyapp ts tys => 1 + tysymbol_size ts + 
-    list_sum (map ty_size tys)
-  end.
-Proof.
-  destruct t; simpl; auto.
-Qed.
-
-Definition ty_size_rel (t1 t2: ty) : Prop :=
-  ty_size t1 < ty_size t2.
-
-Lemma ty_size_rel_wf: well_founded ty_size_rel.
-Proof.
-  unfold well_founded. intros.
-  unfold ty_size_rel.
-  apply Inverse_Image.Acc_inverse_image.
-  apply lt_wf.
-Qed.
-
-Definition ty_node_size_rel (t1 t2: ty) : Prop :=
-  ty_node_size (t1.(ty_node)) < ty_node_size (t2.(ty_node)).
-
-Lemma ty_node_size_rel_wf: well_founded ty_node_size_rel.
-Proof.
-  unfold well_founded. intros.
-  unfold ty_node_size_rel.
-  apply Inverse_Image.Acc_inverse_image.
-  apply lt_wf.
-Qed.
-
-End TySize.
-
-(*Obligations for function def:*)
-
-Lemma node_lt_ty (t: ty):
-  ty_node_size (ty_node t) < ty_size t.
-Proof.
-  unfold ty_size. lia.
-Qed.
-
-Lemma in_tys_lt_app {t ts tys}:
-  ty_node_size (Tyapp ts tys) < ty_size t ->
-  Forall (fun x => ty_size_rel x t) tys.
-Proof.
-  rewrite ty_node_size_rewrite. intros.
-  intros.
-  rewrite List.Forall_forall; intros x Hinx.
-  unfold ty_size_rel.
-  pose proof (in_split x tys Hinx) as Hsplit.
-  destruct Hsplit as [l1 [l2 Htys]]; subst.
-  revert H.
-  rewrite map_app. simpl map.
-  rewrite list_sum_app. simpl list_sum.
-  intros.
-  unfold ty_size at 1. lia.
-Qed.
-
-Section TyBuildSimpl.
-
-Variable (A: Type)(B: Type).
-
-Variable (Hvar: tvsymbol -> A).
-Variable (Happ: tysymbol -> list ty -> B -> A).
-
-Variable (base: B).
-Variable (combine: A -> B -> B).
-
-Fixpoint ty_build_simpl' (t: ty) (ACC: Acc ty_size_rel t) {struct ACC} : A :=
-  match t.(ty_node) as n return ty_node_size n < ty_size t -> A with
-  | Tyvar v => fun _ => Hvar v
-  | Tyapp ts tys => fun Hlt => Happ ts tys
-    ((fix tys_fold (l: list ty) (Hall: Forall (fun x => ty_size_rel x t) l) : B :=
-      match l as l' return Forall (fun x => ty_size_rel x t) l' -> B with
-      | nil => fun _ => base
-      | x :: xs => fun Hall => 
-        combine (ty_build_simpl' x (Acc_inv ACC _ (Forall_inv Hall))) 
-        (tys_fold xs (Forall_inv_tail Hall))
-      end Hall) tys (in_tys_lt_app  Hlt))
-  end (node_lt_ty t).
-
-Definition ty_build_simpl t := ty_build_simpl' t (ty_size_rel_wf t).
-
-(*One theorem we need for using this:*)
-
-Lemma ty_size_rel_node_rel (t1 t2: ty):
-  ty_size_rel t1 t2 <-> ty_node_size_rel t1 t2.
-Proof.
-  unfold ty_size_rel, ty_size, ty_node_size_rel. lia.
-Qed.
-
-Lemma ty_build_simpl_irrel t ACC1 ACC2:
-  ty_build_simpl' t ACC1 = ty_build_simpl' t ACC2.
-Proof.
-  induction t using (well_founded_induction ty_node_size_rel_wf).
-  destruct ACC1; destruct ACC2.
-  simpl.
-  destruct t as [n tg]; simpl. destruct n; auto.
-  f_equal.
-  generalize dependent (in_tys_lt_app (node_lt_ty {| ty_node := Tyapp t l; ty_tag := tg |})).
-  generalize dependent {| ty_node := Tyapp t l; ty_tag := tg |}.
-  induction l; simpl; auto.
-  intros. erewrite IHl. f_equal.
-  apply H.
-  inversion f; subst.
-  apply ty_size_rel_node_rel. auto.
-  auto.
-Qed.
-
-(*And the rewrite lemma:*)
-Lemma ty_build_simpl_rewrite (t: ty) :
-  ty_build_simpl t =
-  match t.(ty_node) with
-        | Tyvar v => Hvar v
-        | Tyapp ts tys => Happ ts tys 
-            (fold_right (fun x acc => combine (ty_build_simpl x) acc) base tys)
-  end.
-Proof.
-  unfold ty_build_simpl at 1.
-  generalize dependent (ty_size_rel_wf t).
-  intros a. destruct a.
-  destruct t as [n tg].
-  destruct n; [reflexivity |].
-  simpl. f_equal.
-  (*Problem: have l in Forall*)
-  generalize dependent (in_tys_lt_app (node_lt_ty {| ty_node := Tyapp t l; ty_tag := tg |})).
-  generalize dependent {| ty_node := Tyapp t l; ty_tag := tg |}.
-  intros t' a'.
-  induction l; simpl; auto.
-  intros.
-  rewrite IHl.
-  f_equal.
-  apply ty_build_simpl_irrel.
-Qed.
-
-End TyBuildSimpl.
-
-(*More general functions*)
-
-(*Do same with Type so that we can write functions and test extraction*)
-
-Definition type_def_p_ty (P: ty -> Type) (t: type_def ty_) : Type :=
-  match t with
-  | Alias _ x => P x
-  | _ => True
-  end.
-
-
-Inductive ForallT {A: Type} (P: A -> Type) : list A -> Type :=
-  | ForallT_nil: ForallT P nil
-  | ForallT_cons: forall {x: A} {l: list A},
-    P x -> ForallT P l -> ForallT P (x :: l).
-
-Lemma ForallT_hd {A: Type} (P: A -> Type) (x: A) (l: list A):
-  ForallT P (x :: l) ->
-  P x.
-Proof.
-  intros. inversion X; subst. apply X0.
-Qed.
-
-Lemma ForallT_tl {A: Type} (P: A -> Type) (x: A) (l: list A):
-  ForallT P (x :: l) ->
-  ForallT P l.
-Proof.
-  intros. inversion X; auto.
-Qed.
-
-Lemma ForallT_In {A: Type} (P: A -> Type)
-  (eq_dec: forall (x y: A), {x = y} + {x <> y}) (l: list A):
-  ForallT P l ->
-  forall x, In x l -> P x.
-Proof.
-  intros Hall. induction Hall; simpl; intros.
-  destruct H.
-  destruct (eq_dec x x0); subst; auto.
-  apply IHHall. destruct H; subst; auto.
-  contradiction.
-Qed.
-
-Lemma typesym_lt_node (ts: tysymbol) (tys: list ty):
-  tysymbol_size ts < ty_node_size (Tyapp ts tys).
-Proof.
-  rewrite ty_node_size_rewrite.
-  lia.
-Qed.
-
-
-Section TyRect.
-
-Variable (P: ty -> Type).
-Variable (P1: ty_node_ -> Type).
-Variable (P2: tysymbol -> Type).
-
-Variable (Hty: forall (t: ty), P1 (t.(ty_node)) -> P t).
-Variable (Hsym: forall (ts: tysymbol), type_def_p_ty P (ts.(ts_def)) ->
-  P2 ts).
-Variable (Hvar: forall v, P1 (Tyvar v)).
-Variable (Happ: forall ts tys, P2 ts -> ForallT P tys -> P1 (Tyapp ts tys)).
-
-(*This does NOT work - tysymbol is not recursive so we can't have
-  a fixpoint on it
-  Maybe could do same trick (assume we have proof, populate later)
-  but likely to run into positivity problems*)
-
-
-(*Fixpoint gcd_rec (a b: nat) (ACC: Acc lt b) {struct ACC} : nat :=
-  if Nat.eq_dec b 0 then a else gcd_rec b (a mod b) (Acc_inv ACC _).*)
-
-(*TODO: need decomposition if we want idiomatic code, maybe need eq_rect*)
-(*Plan: prove lemmas, do in Set, test extraction (without Program) *)
-Fixpoint ty_rect' (t: ty) (ACC: Acc lt (ty_size t)) {struct ACC} : P t :=
-  (Hty t (ty_node_rect' t.(ty_node) 
-    (Acc_inv ACC (ty_node_size (ty_node t)) (node_lt_ty t))))
-with ty_node_rect' (t: ty_node_) (ACC: Acc lt (ty_node_size t)) {struct ACC} : P1 t :=
-  match t as t' return Acc lt (ty_node_size t') -> P1 t' with
-  | Tyvar tv => fun _ => Hvar tv
-  | Tyapp ts tys => fun ACC => Happ ts tys (tysymbol_rect' ts (Acc_inv ACC (tysymbol_size ts) 
-      (typesym_lt_node ts tys))) 
-    ((fix tys_rect (l: list ty) 
-      (Hl: Forall (fun x => ty_size x < (ty_node_size (Tyapp ts tys))) l) 
-      : ForallT P l :=
-      match l as l' return Forall  (fun x => ty_size x < (ty_node_size (Tyapp ts tys))) l'->
-        ForallT P l'  with
-      | nil => fun _ => ForallT_nil _
-      | x :: xs => fun Hl => ForallT_cons _ (ty_rect' x (Acc_inv ACC (ty_size x) 
-        (List.Forall_inv Hl))) 
-        (tys_rect xs (List.Forall_inv_tail Hl))
-      end Hl) tys (in_tys_lt_app ts tys))
-  end ACC
-with tysymbol_rect' (ts: tysymbol) (ACC: Acc lt (tysymbol_size ts)) {struct ACC} : P2 ts :=
-  Hsym ts (
-    match (ts.(ts_def)) as d' return type_def_size d' < tysymbol_size ts -> 
-       type_def_p_ty P d' with
-    | NoDef _ => fun _ => I
-    | Alias _ x => fun Hlt => ty_rect' x (Acc_inv ACC (ty_size x) (alias_lt_sym Hlt))
-    end (def_lt_sym ts)
-  ).
-
-Definition ty_rect (t: ty) : P t := ty_rect' t (lt_wf _).
-Definition ty_node_rect (t: ty_node_) : P1 t := ty_node_rect' t (lt_wf _).
-Definition tysymbol_rect (ts: tysymbol) : P2 ts := tysymbol_rect' ts (lt_wf _).
-
-End TyRect.
-
-(*Example (TODO move)*)
-Definition ty_v_map (f: tvsymbol -> ty) (t: ty) : ty :=
-  ty_build_simpl ty (list ty) (fun v => f v)
-  (fun ts tys res => Build_ty_ _ (Tyapp ts res) CoqBigInt.zero) 
-  nil cons t.
-Print type_def.
-
-(*For equality, we have to do things manually*)
-Fixpoint ty_eqb (t1 t2: ty) (ACC: Acc ty_size_rel t1) {struct ACC} :=
-  ty_node_eqb t1.(ty_node) t2.(ty_node) &&
-  CoqBigInt.eq t1.(ty_tag) t2.(ty_tag) 
-with ty_node_eqb (t1 t2: ty_node) (ACC: Acc ty_node_size_rel t1) {struct ACC} :=
+Lemma ty_eqb_rewrite t1 t2:
+  ty_eqb t1 t2 =
   match t1, t2 with
-  | Tyvar v1, Tyvar v2 => tvsymbol_eqb v1 v2
-  | Tyapp ts1 tys1, Tyapp ts2 tys2 =>
-    tysymbol_eqb ts1 ts2 &&
-    ((fix tys_eqb (l1 l2: list ty) : bool :=
-      match l1, l2 with
-      | h1 :: tl1, h2 :: tl2 => ty_eqb h1 h2 && tys_eqb tl1 tl2
-      | nil, nil => true
-      | _, _ => false
-      end) tys1 tys2)
-  | _, _ => false
-  end
-with tysymbol_eqb (ts1 ts2: tysymbol) (ACC: Acc tysymbol_size_rel t1) {struct ACC} :=
-  ident_eqb t1.(ts_name) t2.(ts_name) &&
-  list_eqb tvsymbol_eqb t1.(ts_args) t2.(ts_args) &&
-
-
-
-
-Record ty_ (A: Type) := 
-  { ty_node: A;
-    ty_tag: CoqBigInt.t}.
-
-
-
-Fixpoint ty_build_simpl' (t: ty) (ACC: Acc ty_size_rel t) {struct ACC} : A :=
-  match t.(ty_node) as n return ty_node_size n < ty_size t -> A with
-  | Tyvar v => fun _ => Hvar v
-  | Tyapp ts tys => fun Hlt => Happ ts tys
-    ((fix tys_fold (l: list ty) (Hall: Forall (fun x => ty_size_rel x t) l) : B :=
-      match l as l' return Forall (fun x => ty_size_rel x t) l' -> B with
-      | nil => fun _ => base
-      | x :: xs => fun Hall => 
-        combine (ty_build_simpl' x (Acc_inv ACC _ (Forall_inv Hall))) 
-        (tys_fold xs (Forall_inv_tail Hall))
-      end Hall) tys (in_tys_lt_app  Hlt))
-  end (node_lt_ty t).
-
-
-(*This almost works, but not quite, because our function
-  schema is not specific enough*)
-(*Definition ty_eqb (t1 t2: ty) : bool :=
-  (ty_build_simpl (ty -> bool) (list ty -> bool) (fun v t2 => 
-    match t2.(ty_node) with
-    | Tyvar v2 => typevar_eqb v v2
-    | _ => false
-    end) 
-    (fun ts tys res t2 => match t2.(ty_node) with
-    | Tyapp ts1 tys2 => tysymbol_eqb ts ts1 &&
-      res tys2
-    | _ => false
-    end) 
-    (*Base*)
-    (fun l =>
-      match l with 
-      | nil => true
-      | _ => false
-      end)
-    (*combine*)
-    (fun fhd ftl =>
-      fun l => match l with
-                | hd1 :: tl1 => fhd hd1 && ftl tl1
-                | _ => false
-      end)) t1 t2.*)
-From Equations Require Import Equations.
-Section TestEq.
-
-Variable (f: tvsymbol -> ty).
-(*Let's try with Equations and see how the resulting OCaml code is*)
-Equations ty_v_map' (t: ty) : ty by
-  struct t
-  (*wf (ty_size t) lt*) :=
-  ty_v_map' t := ty_v_map_node t.(ty_node)
-where ty_v_map_node (t: ty_node_) : ty by
-  struct t
-  (*wf (ty_node_size t) lt*) :=
-  ty_v_map_node (Tyvar v) := f v;
-  ty_v_map_node (Tyapp ts tys) :=
-    Build_ty_ _ (Tyapp ts (List.map (ty_v_map') tys)) xH.
-
-
-    ty_app f (List.map (ty_v_map fn) tl)
-
-
-  (list ty) (fun v => f v)
-  (fun ts tys res => Build_ty_ _ (Tyapp ts res) xH) 
-  nil cons t.
-
-
-
-ty_v_map (f: tvsymbol -> ty) (t: ty) : ty :=
-  ty_build_simpl ty (list ty) (fun v => f v)
-  (fun ts tys res => Build_ty_ _ (Tyapp ts res) xH) 
-  nil cons t.
-    
-    ) (fun )
-
-
-  (fun ts tys res => res)
-
-(*Now let's try a 2-argument one, of the form:
-  let rec foo (t1 t2: ty) =
-  match t1.ty_node, t2.ty_node with
-  | Tyvar v1, Tyvar v2 => f1 v1 v2
-  | Tyapp ts1 tys1, Tyapp ts2 tys2 => f2 ts1 tys1 ts2 tys2
-  *)
-
-
-(*Writing functions on types*)
-
-(*Decidable equality on types*)
-
-
-
-(*TODO: not best way*)
-(*
-Module Type Ty (I: Ident).
-
-(*Type variables*)
-Record tvsymbol := {
-  tv_name : I.ident
-}.
-
-(*TODO: add range and float*)
-Inductive type_def (A: Set) : Set :=
-  | NoDef
-  | Alias: A -> type_def A.
-
-(*Fail Inductive tysymbol := {
-  ts_name : I.ident;
-  ts_args : list tvsymbol;
-  ts_def: type_def ty
-}
-with ty := {
-  ty_node : ty_node;
-  ty_tag : tag
-}
-with ty_node_ :=
-  | Tyvar : tvsymbol -> ty_node_
-  | Tyapp : tysymbol -> list ty -> ty_node_.*)
-
-
-(*1 version:
-*)
-Inductive tysymbol : Set :=
-  | mk_tysymbol : I.ident -> list tvsymbol -> type_def ty -> tysymbol 
-with ty : Set :=
-  | mk_ty : ty_node_ -> tag -> ty
-with ty_node_ : Set :=
-  | Tyvar : tvsymbol -> ty_node_
-  | Tyapp : tysymbol -> list ty -> ty_node_.
-
-
-(*Simulate record but not as good*)
-Parameter ts_name : tysymbol -> I.ident.
-Parameter ts_args : tysymbol -> list tvsymbol.
-Parameter ts_def : tysymbol -> type_def ty.
-
-Parameter ty_node: ty -> ty_node_.
-Parameter ty_tag: ty -> tag.
-
-(*A few examples*)
-Parameter ts_equal: tysymbol -> tysymbol -> bool.
-(*Parameter ty_equal: ty -> ty -> bool.*)
-
-End Ty.
-
-Module TyImpl (I: Ident) <: Ty I.*)
-
-(*Type variables*)
-Record tvsymbol := {
-  tv_name : ident
-}.
-
-
-
-(*Unset Elimination Schemes.
-Inductive tysymbol : Set :=
-  | mk_tysymbol : ident -> list tvsymbol -> type_def ty -> tysymbol 
-with ty : Set :=
-  | mk_ty : ty_node_ -> tag -> ty
-with ty_node_ : Set :=
-  | Tyvar : tvsymbol -> ty_node_
-  | Tyapp : tysymbol -> list ty -> ty_node_.
-Set Elimination Schemes.
-
-Scheme tysymbol_ind := Induction for tysymbol Sort Prop with
-ty_ind := Induction for ty Sort Prop with
-ty_node__ind := Induction for ty_node_ Sort Prop.
-
-Check ty_ind.*)
-
-
-
-
-(*Test*)
-
-(*This awkward definition satisfies Coq's positivity checker
-  for nested induction, unlike the normal one*)
-Definition map2 {A B C: Type} :=
-  fun (f: A -> B -> C) =>
-    fix map2 (l1: list A) : list B -> list C :=
-      match l1 with
-      | nil => fun l2 => nil
-      | x1 :: t1 =>
-        fun l2 =>
-        match l2 with
-        | nil => nil
-        | x2 :: t2 => f x1 x2 :: map2 t1 t2
-        end
-      end.
-
-(*This doesn't work, let's try to prove induction principle*)
-Fail Fixpoint ty_equal (t1 t2: ty) {struct t1} : bool :=
-  match t1.(ty_node), t2.(ty_node) with
-  | Tyvar v1, Tyvar v2 => true
-  | Tyapp ts1 tys1, Tyapp ts2 tys2 => 
-    forallb (fun x => x) (map2 ty_equal tys1 tys2)
-  | _, _ => false
+  | mk_ty n1 i1, mk_ty n2 i2 =>
+    CoqBigInt.eqb i1 i2 && ty_node_eqb n1 n2
   end.
-
-
-Definition type_def_p (P: ty -> Prop) (t: type_def ty_) : Prop :=
-  match t with
-  | NoDef _ => True
-  | Alias _ x => P x
-  end.
-
-Section TyInd.
-
-Variable (P: ty -> Prop).
-Variable (P1: ty_node_ -> Prop).
-Variable (P2: tysymbol -> Prop).
-
-Variable (Hty: forall n t, P1 n -> P (Build_ty_ _ n t)).
-Variable (Hsym: forall n vs t, type_def_p P t -> P2 (Build_tysymbol_ _ n vs t)).
-Variable (Hvar: forall v, P1 (Tyvar v)).
-Variable (Happ: forall ts tys, P2 ts -> Forall P tys -> P1 (Tyapp ts tys)).
-
-(*This does NOT work - tysymbol is not recursive so we can't have
-  a fixpoint on it
-  Maybe could do same trick (assume we have proof, populate later)
-  but likely to run into positivity problems*)
-
-Fail Fixpoint ty_ind (t: ty) : P t :=
-  match t with
-  | Build_ty_ _ n tg => Hty n tg (ty_node_ind n)
-  end
-with ty_node_ind (t: ty_node_) : P1 t :=
-  match t with
-  | Tyvar tv => Hvar tv
-  | Tyapp ts tys => Happ ts tys (tysymbol_ind ts) 
-    ((fix tys_ind (l: list ty) : Forall P l :=
-      match l with
-      | nil => List.Forall_nil _
-      | x :: xs => List.Forall_cons _ _ _ (ty_ind x) (tys_ind xs)
-      end) tys)
-  end
-with tysymbol_ind (ts: tysymbol) : P2 ts :=
-  match ts with
-  | Build_tysymbol_ _ n l d => Hsym n l d 
-    (match d as d' return type_def_p P d' with
-      | NoDef _ => I
-      | Alias _ x => ty_ind x
-    end)
-  end.
-
-End TyInd.
-
-(*Let's try bad*)
-Inductive func {A: Set} : Set :=
-  | func1: (A -> A) -> func.
-
-Fail Inductive bad : Set :=
-  | bad1: @func bad -> bad.
-
-(*Next: structural recursion on size*)
-
-
-(*Need version of map2 with in*)
-Definition map2' {A B C: Type} :=
-    fix map2 (l1: list A) : list B -> (A -> B -> C) -> list C :=
-      match l1 with
-      | nil => fun l2 f => nil
-      | x1 :: t1 =>
-        fun l2 f =>
-        match l2 with
-        | nil => nil
-        | x2 :: t2 => f x1 x2 :: map2 t1 t2 f
-        end
-      end.
-
-Definition map2'' {A B C: Type} :=
-    fix map2 (l1: list A) : forall (l2: list B), 
-      (forall (x: A) (Hinx: In x l1) (y: B) (Hiny: In y l2), C) -> list C :=
-      match l1 with
-      | nil => fun l2 f => nil
-      | x1 :: t1 =>
-        fun l2 =>
-        match l2 with
-        | nil => fun f => nil
-        | x2 :: t2 => fun f => f x1 (in_eq _ _) x2 (in_eq _ _) :: map2 t1 t2 
-          (fun x Hin y Hin2 => f x (in_cons _ _ _ Hin) y (in_cons _ _ _ Hin2))
-        end
-      end.
-
-Definition type_def_size (t: type_def ty) : nat :=
-  match t with
-  | NoDef _ => 0
-  | Alias _ x => 1 + ty_size x
-  end.
-
-
-(*Obligations (do here to test OCaml)*)
-
-
-Lemma ty_decomp (t: ty):
-{| ty_node := ty_node t; ty_tag := ty_tag t |} = t.
 Proof.
-  destruct t; reflexivity.
+  destruct t1; destruct t2; reflexivity.
 Qed.
 
-
-(*Lemma foo (x: nat) x < x + 1.
-
-Lemma bar (x y: nat) : x < y -> y > x.*)
-
-Lemma in_tys_lt_app (ts: tysymbol) (tys: list ty) :
-Forall (fun x : ty => ty_size x < ty_node_size (Tyapp ts tys)) tys.
+Lemma ty_eqb_eq_aux: 
+  (forall t1 t2, t1 = t2 <-> ty_eqb t1 t2) /\
+  (forall t1 t2, t1 = t2 <-> ty_node_eqb t1 t2) /\
+  (forall t1 t2, t1 = t2 <-> tysymbol_eqb t1 t2).
 Proof.
-  (*TODO: bad proof*)
-  rewrite ty_node_size_rewrite.
-  rewrite List.Forall_forall; intros x Hinx.
-  pose proof (in_split x tys Hinx) as Hsplit.
-  destruct Hsplit as [l1 [l2 Htys]]; subst.
-  rewrite map_app; simpl.
-  rewrite list_sum_app. simpl. unfold ty_size at 1. lia.
-Qed.
-
-Lemma alias_lt_sym {x ts}:
-type_def_size (Alias ty_ x) < tysymbol_size ts ->
-ty_size x < tysymbol_size ts.
-Proof.
-  simpl. lia.
-Qed.
-
-Lemma def_lt_sym ts: type_def_size (ts_def ts) < tysymbol_size ts.
-Proof.
-  unfold tysymbol_size; simpl.
-  destruct (ts_def ts); auto.
-Qed.
-
-(*Let's try to prove an induction principle*)
-
-Section TyInd.
-
-Variable (P: ty -> Prop).
-Variable (P1: ty_node_ -> Prop).
-Variable (P2: tysymbol -> Prop).
-
-Variable (Hty: forall (t: ty), P1 (t.(ty_node)) -> P t).
-Variable (Hsym: forall (ts: tysymbol), type_def_p P (ts.(ts_def)) ->
-  P2 ts).
-Variable (Hvar: forall v, P1 (Tyvar v)).
-Variable (Happ: forall ts tys, P2 ts -> Forall P tys -> P1 (Tyapp ts tys)).
-
-(*This does NOT work - tysymbol is not recursive so we can't have
-  a fixpoint on it
-  Maybe could do same trick (assume we have proof, populate later)
-  but likely to run into positivity problems*)
-
-
-(*Fixpoint gcd_rec (a b: nat) (ACC: Acc lt b) {struct ACC} : nat :=
-  if Nat.eq_dec b 0 then a else gcd_rec b (a mod b) (Acc_inv ACC _).*)
-
-(*TODO: need decomposition if we want idiomatic code, maybe need eq_rect*)
-(*Plan: prove lemmas, do in Set, test extraction (without Program) *)
-Fixpoint ty_ind' (t: ty) (ACC: Acc lt (ty_size t)) {struct ACC} : P t :=
-  (Hty t (ty_node_ind' t.(ty_node) 
-    (Acc_inv ACC (ty_node_size (ty_node t)) (node_lt_ty t))))
-with ty_node_ind' (t: ty_node_) (ACC: Acc lt (ty_node_size t)) {struct ACC} : P1 t :=
-  match t as t' return Acc lt (ty_node_size t') -> P1 t' with
-  | Tyvar tv => fun _ => Hvar tv
-  | Tyapp ts tys => fun ACC => Happ ts tys (tysymbol_ind' ts (Acc_inv ACC (tysymbol_size ts) 
-      (typesym_lt_node ts tys))) 
-    ((fix tys_ind (l: list ty) 
-      (Hl: Forall (fun x => ty_size x < (ty_node_size (Tyapp ts tys))) l) 
-      : Forall P l :=
-      match l as l' return Forall  (fun x => ty_size x < (ty_node_size (Tyapp ts tys))) l'->
-        Forall P l'  with
-      | nil => fun _ => List.Forall_nil _
-      | x :: xs => fun Hl => List.Forall_cons _ _ _ (ty_ind' x (Acc_inv ACC (ty_size x) 
-        (List.Forall_inv Hl))) 
-        (tys_ind xs (List.Forall_inv_tail Hl))
-      end Hl) tys (in_tys_lt_app ts tys))
-  end ACC
-with tysymbol_ind' (ts: tysymbol) (ACC: Acc lt (tysymbol_size ts)) {struct ACC} : P2 ts :=
-  Hsym ts (
-    match (ts.(ts_def)) as d' return type_def_size d' < tysymbol_size ts -> 
-       type_def_p P d' with
-    | NoDef _ => fun _ => I
-    | Alias _ x => fun Hlt => ty_ind' x (Acc_inv ACC (ty_size x) (alias_lt_sym Hlt))
-    end (def_lt_sym ts)
-  ).
-
-Definition ty_ind (t: ty) : P t := ty_ind' t (lt_wf _).
-Definition ty_node_ind (t: ty_node_) : P1 t := ty_node_ind' t (lt_wf _).
-Definition tysymbol_ind (ts: tysymbol) : P2 ts := tysymbol_ind' ts (lt_wf _).
-
-End TyInd.
-
-
-
-
-(*Alternate version, more useful*)
-Section TyBuild.
-
-(*First is for ty, second is for ty_node_*)
-Variable (A: Type) (B: Type) (C: Type).
-
-(*type, result of calling function on t.ty_node, result*)
-Variable (Hty: ty -> B -> A).
-Variable (Hvar: tvsymbol -> B).
-(*TODO: not general enough probably*)
-(*3rd param: folding over the resulting list*)
-Variable (base: C).
-Variable (combine: C -> A -> C).
-(*B is result of fold over list of tys*)
-Variable (Happ: tysymbol -> list ty -> C -> B).
-
-Fixpoint ty_build' (t: ty) (ACC: Acc lt (ty_size t)) {struct ACC} : A :=
-  (Hty t (ty_node_build' t.(ty_node)
-    (Acc_inv ACC (ty_node_size (ty_node t)) (node_lt_ty t))))
-with ty_node_build' (t: ty_node_) (ACC: Acc lt (ty_node_size t)) {struct ACC} : B :=
-  match t as t' return Acc lt (ty_node_size t') -> B with
-  | Tyvar tv => fun _ => Hvar tv
-  | Tyapp ts tys => fun ACC => Happ ts tys
-    (*Here, we implement fold*)
-    ((fix tys_fold (l: list ty) 
-      (Hl: Forall (fun x => ty_size x < (ty_node_size (Tyapp ts tys))) l) 
-      : C :=
-      match l as l' return Forall  (fun x => ty_size x < (ty_node_size (Tyapp ts tys))) l'->
-        C  with
-      | nil => fun _ => base
-      | x :: xs => fun Hl => combine (tys_fold xs (List.Forall_inv_tail Hl))
-          (ty_build' x (Acc_inv ACC (ty_size x) 
-        (List.Forall_inv Hl)))
-      end Hl) tys (in_tys_lt_app ts tys))
-  end ACC.
-
-Definition ty_build (t: ty) := ty_build' t (lt_wf _).
-Definition ty_node_build (t: ty_node_) := ty_node_build' t (lt_wf _).
-
-
-End TyBuild.
-
-
-  
-
-
-(*TODO: prove this later*)
-(*Ltac hide_right := match goal with |- _ = ?rhs =>remember rhs end. 
-
-Lemma ty_build_rewrite (t: ty):
-  ty_build t =
-  Hty t (match t.(ty_node) with
-        | Tyvar v => Hvar v
-        | Tyapp ts tys => Happ ts tys 
-            (fold_right (fun x acc => combine acc (ty_build x)) base tys)
-  end).
-Proof.
-  unfold ty_build.
-  destruct (lt_wf (ty_size t)) as [a].
-  simpl ty_build' at 1. f_equal.
-  generalize dependent (a (ty_node_size (ty_node t)) (node_lt_ty t)).
-  intros a1.
-  destruct a1. 
-  
-
-  
-   unfold ty_node_build'. cbv beta. cbv. simpl ty_node_build' at 1.
-  destruct t as [n tg].
-  destruct n.
-  - simpl; auto.
-  - hide_right. simpl. subst b.
-    simpl ty_node. cbv iota. f_equal.
-    generalize dependent (in_tys_lt_app t l).
-    induction l; auto.
-    intros Hall. (*TODO: bad hack*) Opaque ty_build'. simpl.
-    f_equal.
-    erewrite <- IHl.
-
-    Unshelve. reflexivity.
-    f_equal.
-
-
-    + auto.
-    + simpl. auto.
-
-
-
-
-  
-  
-   simpl ty_node_build' at 1.
-  destruct t as [n tg].
-  simpl ty_node at 1 2 .
-  simpl.
-
-
-  (*To generalize*)
-  assert (forall (f: forall x : ty_, Acc lt (ty_node_size (ty_node x))),
-    Hty t (ty_node_build' (ty_node t) (a (ty_node_size (ty_node t)) (node_lt_ty t))) =
-    match ty_node t with
-    | 
-
-
-
-
-  generalize dependent (fun x => (Acc_intro (ty_node_size (ty_node x)) (λ (b : nat) (Hb : b < ty_node_size (ty_node x)), nat_ind (λ n : nat, ∀ a0 : nat, a0 < n → Acc (ltof nat (λ m : nat, m)) a0) (λ (a0 : nat) (Ha : a0 < 0), False_ind (Acc (ltof nat (λ m : nat, m)) a0) (PeanoNat.Nat.nlt_0_r a0 Ha)) (λ (n : nat) (IHn : ∀ a0 : nat, a0 < n → Acc (ltof nat (λ m : nat, m)) a0) (a0 : nat) (Ha : a0 < S n), Acc_intro a0 (λ (b0 : nat) (Hb0 : b0 < a0), IHn b0 (PeanoNat.Nat.lt_le_trans b0 a0 n Hb0 (match PeanoNat.Nat.succ_le_mono a0 n with
-| conj _ H0 => H0
-end Ha)))) (ty_node_size (ty_node x)) b (PeanoNat.Nat.lt_le_trans b (ty_node_size (ty_node x)) (ty_node_size (ty_node x)) Hb (match PeanoNat.Nat.succ_le_mono (ty_node_size (ty_node x)) (ty_node_size (ty_node x)) with
-| conj _ H0 => H0
-end (PeanoNat.Nat.lt_le_trans (ty_node_size (ty_node x)) (ty_size x) (ty_size x) (node_lt_ty x) (match PeanoNat.Nat.succ_le_mono (ty_size x) (ty_size x) with
-| conj _ H0 => H0
-end (PeanoNat.Nat.lt_succ_diag_r (ty_size x))))))))).
-
-
-  generalize dependent 
-  Check Acc_intro.
-  match goal with
-  | |- context [Acc_intro ?a ?b ?c ?d] => idtac a
-  end.
-  generalize dependent (a (ty_node_size (ty_node t)) (node_lt_ty t)).
-  destruct t; simpl. intros a1. f_equal.
-  destruct ty_node0; simpl.
-  - destruct a1; auto.
-  - destruct a1; simpl. f_equal.
-  
-  
-   destruct (a 1 (node_lt_ty {| ty_node := Tyvar t; ty_tag := ty_tag0 |})); simpl; auto.
-  - destruct ((a (S (S (match ts_def t with
-| NoDef _ => 0
-| Alias _ x => S (S (ty_node_size (ty_node x)))
-end + list_sum (map (λ x : ty, S (ty_node_size (ty_node x))) l)))))).
-  
-   unfold ty_node_build'; simpl.
-
-  (*generalize dependent (lt_wf (ty_size t)).*)
-  induction t using (well_founded_induction (ty_size_rel_wf)).
-  intros ACC.
-  destruct t as [n tg].
-  inversion ACC.
-  unfold ty_build' at 1. simpl.
-  simpl ty_build'. at 1.
-  simpl at 1.
-  destruct t; simpl in *.
-
-
-
-  revert t.
-  eapply ty_ind with (P1).
-  - intros.
-
-    destruct t0; simpl.
-  
-   with (P:= fun t => forall(a : Acc lt (ty_size t)), ty_build' t a = Hty t match ty_node t with
-| Tyvar v => Hvar v
-| Tyapp ts tys => Happ ts tys (foldr (λ (x : ty) (acc : C), combine acc (ty_build' x (lt_wf (ty_size x)))) base tys)
-end ).
-
-  dependent induction (ty_size t) using (well_founded_induction lt_wf).
-  unfold ty_build'. simpl. 
-        
-        
-        
-        combine base tys))
-
-
-End TyBuild.*)
-
-
-
-
-(*
-Definition ty_v_map (f: tvsymbol -> ty) (t: ty) :=
-  ty_build ty (fun _ x => x) (fun v => f v) (fun ts tys IHl =>
-    Build_ty_ _ (Tyapp ts IHl) xH).
-
-
-Eval compute in 
-
-(*Let us do ty_v_map first*)
-Definition ty_v_map (f: tvsymbol -> ty) (t: ty) :=
-  ty_rect (fun (_: ty) => ty) (fun (_: ty_node) => ty) (fun _ => unit)
-  (*ty case*)
-  (fun (t1: ty) (res: bool) => res)
-  (fun _ _ => tt)
-  (*Tvar*)
-  (fun (v: tvsymbol) => f v)
-  (*Tyapp*)
-  (fun (ts: tysymbol) (tys: list ty) (IH))
-
-(*Common pattern:
-  let rec ty_foo (t1 t2: ty) : A :=
-    match t1.ty_node, t2.ty_node with
-    | *)
-
-(*Test*)
-Fixpoint list_eq (l1 l2: list nat) : bool :=
-  match l1, l2 with
-  | x1 :: t1, x2 :: t2 => Nat.eqb x1 x2 && list_eq t1 t2
-  | nil, nil => true
-  | _, _ => false
-  end.
-
-Definition list_eq' (l1 l2: list nat) : bool.
-revert l2.
-induction l1 as [| x1 t1 eq_t1]; intros l2.
-- destruct l2.
-  + apply true.
-  + apply false.
-- destruct l2 as [| x2 t2].
-  + apply false.
-  + apply (Nat.eqb x1 x2 && eq_t1 t2).
-Defined.
-
-Definition list_eq'' : list nat -> list nat -> bool :=
-  (list_rec (fun (_ : list nat) => list nat -> bool)
-    (*nil case*)
-    (fun l2 => match l2 with
-              | nil => true
-              | _ => false
-    end)
-    (*cons case*)
-    (fun x1 t1 (IH: list nat -> bool) (l2: list nat) =>
-      match l2 with
-      | nil => false
-      | x2 :: t2 => Nat.eqb x1 x2 && IH t2
-      end
-    )).
-(*NOTE: I think we DONT want ForallT, maybe want fixpoint instead but see*)
-(*NOTE: want version without tysymbol*)
-(*Now we can define an equality function (maybe)*)
-Definition ty_equal (t1 t2: ty) : bool :=
-  ty_rect (fun (_: ty) => ty -> bool ) (fun (_: ty_node_ ) => ty_node_ -> bool) 
-    (fun _ => unit)
-  (*ty case*)
-  (fun (t1: ty) (node_eq: ty_node_ -> bool) (t2: ty) =>
-    node_eq (t2.(ty_node))
-  )
-  (*tysymbol case*)
-  (fun (ts1: tysymbol) _ => tt)
-  (*ty_node_ Tyvar case*)
-  (fun (v1: tvsymbol) (t2: ty_node_) =>
-    match t2 with
-    | Tyvar v2 => true (*TODO*)
-    | _ => false
-    end) 
-  (*ty_node_ Tyapp case*)
-  (fun (ts: tysymbol) (tys: list ty) (_: unit) IH (t2: ty_node_) =>
-    match t2 with
-    | Tyvar v2 => false
-    | Tyapp ts2 tys2 => IH tys2 (*nope*)
-    end)
-  
-  .
-
-
-
-
-
-
-  ty_rect (fun _ => ty -> bool) (fun _ => ty_node_ -> bool) (fun _ => unit) t1.
-
-
-
-
-
-
-Next Obligation.
-intros. subst. unfold ty_size. simpl. apply Nat.lt_succ_diag_r.
-Qed.
-Next Obligation.
-intros. subst. rewrite ty_node_size_rewrite.
-(*bad*) lia.
-Qed.
-Next Obligation.
-intros. subst. apply Forall_inv in Hl. assumption.
-Defined.
-Next Obligation.
-intros.
-subst. apply Forall_inv_tail in Hl; assumption.
-Defined.
-Next Obligation.
-intros.
-rewrite List.Forall_forall.
-(*Not great proof*)
-clear; intros.
-rewrite ty_node_size_rewrite.
-pose proof (in_split x tys H).
-destruct H0 as [l1 [l2 Htys]]; subst.
-rewrite map_app; simpl.
-rewrite list_sum_app. simpl. unfold ty_size at 1. lia.
-Qed.
-Next Obligation.
-intros. subst.
-simpl in Hlt. lia.
-Qed.
-Next Obligation.
-intros. subst. unfold tysymbol_size. simpl.
-destruct d; simpl; auto.
-Qed.
-
-
-Record tysymbol_ (A: Set) : Set := {
-  ts_name : ident;
-  ts_args : list tvsymbol;
-  ts_def : type_def (@ty_ A)
-}.
- 
-
-Search In
-rewrite Forall_forall.
-intros.
-
-clear. induction tys; simpl; auto.
-constructor; auto.
-- 
-
-
-subst.
-
-
- Search Forall. rewrite ty_node_size_rewrite.
-
- simpl.
-
- Search (?x < S ?x). 
-
-
-End TyInd.
-
-(*Now can we do proof on Acc?*)
-Fixpoint ty_equal (t1 t2: ty) (ACC: Acc lt (ty_size t1)) {struct ACC} : bool :=
-  match t1.(ty_node), t2.(ty_node) with
-  | Tyvar v1, Tyvar v2 => true
-  | Tyapp ts1 tys1, Tyapp ts2 tys2 => 
-    forallb (fun x => x) (map2'' tys1 tys2
-      (fun x Hinx y Hiny => ty_equal x y (Acc_inv _ _ _)))
-  | _, _ => false
-  end.
-
-
-  do 3 f_equal.
-  induction l; simpl; auto.
-  rewrite IHl. reflexivity.
-  f_equal. f_equal. f_equal.
-  unfold ty_node_size.
-    (1 + match (ts_def ts) with
-          | NoDef _ => 0
-          | Alias _ x => 1 + (1 + ty_node_size (x.(ty_node)))
-    end) +
-  
-   fold_right plus 0 
-      (map (fun (x: ty) => ty_node_size (x.(ty_node))) tys)
-  end.
-
-Print tysymbol_.
-
-Definition ty_size {A: Type} (sz: A -> nat)
-
-
-
-
-Definition ty_size {A: Type} (sz: A -> nat) (t: @ty_ A) : nat :=
-
-
-
-
-
-Print tysymbol_.
-
-
-Print ty_.
-
-Print ty_node_.
-
-Variable ()
-    
-
-
-(*Fail Inductive tysymbol := {
-  ts_name : I.ident;
-  ts_args : list tvsymbol;
-  ts_def: type_def ty
-}
-with ty := {
-  ty_node : ty_node;
-  ty_tag : tag
-}
-with ty_node_ :=
-  | Tyvar : tvsymbol -> ty_node_
-  | Tyapp : tysymbol -> list ty -> ty_node_.*)
-
-
-(*1 version:
-*)
-(*Inductive tysymbol : Set :=
-  | mk_tysymbol : ident -> list tvsymbol -> type_def ty -> tysymbol 
-with ty : Set :=
-  | mk_ty : ty_node_ -> tag -> ty
-with ty_node_ : Set :=
-  | Tyvar : tvsymbol -> ty_node_
-  | Tyapp : tysymbol -> list ty -> ty_node_.
-
-Definition ts_name (t: tysymbol) : ident :=
-  match t with
-  | mk_tysymbol i _ _ => i
-  end.
-
-Definition ts_args (t: tysymbol) : list tvsymbol :=
-  match t with
-  | mk_tysymbol _ l _ => l
-  end.
-
-Definition ts_def (t: tysymbol) : type_def ty :=
-  match t with
-  | mk_tysymbol _ _ t => t
-  end.
-
-Definition ty_node (t: ty) : ty_node_ :=
-  match t with
-  | mk_ty t _ => t
-  end.
-
-Definition ty_tag (t: ty) : tag :=
-  match t with
-  | mk_ty _ t => t
-  end.*)
-  
-(*ts_equal and ty_equal are reference equality in OCaml impl*)
-Definition ts_equal (t1 t2: tysymbol) : bool :=
-  id_equal (ts_name _ t1) (ts_name _ t2).
-
-(*End TyImpl.*)
-
-*)
-
-
-
-
-
-
-
-
-
-
-
-
-
-
-*)
+  apply ty_mut_ind.
+  - intros t IH t2.
+    rewrite ty_eqb_rewrite.
+    destruct t as [n1 i1]; destruct t2 as [n2 i2]; simpl in *.
+    rewrite andb_true, <- IH, <- CoqBigInt.eqb_eq.
+    solve_eqb_eq.
+  - intros. simpl. destruct t2 as [v2 |]; [| split; discriminate].
+    rewrite <- tvsymbol_eqb_eq. solve_eqb_eq.
+  - intros ts tys IHsym IHl.
+    simpl.
+    destruct t2 as [v2 | ts1 tys2]; [split;discriminate |].
+    rewrite !andb_true, <- IHsym.
+    destruct (Nat.eqb_spec (length tys) (length tys2)) as [Hlen| Hlen];
+    [| solve_eqb_eq].
+    (*TODO: maybe separate lemma*)
+    assert (Hl: tys = tys2 <-> forallb id (map2 ty_eqb tys tys2)). {
+      clear -IHl Hlen.
+      generalize dependent tys2.
+      induction tys as [| thd ttl IHtys]; simpl; intros [|th2 ttl2];
+      try solve[split; solve[auto; discriminate]].
+      simpl. intros Hlen.
+      rewrite andb_true, <- (Forall_inv IHl th2), <- IHtys; auto.
+      - solve_eqb_eq.
+      - apply Forall_inv_tail in IHl; assumption.
+    }
+    rewrite <- Hl. solve_eqb_eq.
+  - intros [i vs d]; simpl; intros IH [i1 vs2 d2]; simpl.
+    rewrite !andb_true, <- ident_eqb_eq, <- (list_eqb_eq tvsymbol_eqb_eq).
+    destruct d; destruct d2; simpl; try solve_eqb_eq.
+    (*3 interesting cases*)
+    + rewrite <- IH. solve_eqb_eq.
+    + rewrite <- Number.int_range_eqb_eq. solve_eqb_eq.
+    + rewrite <- Number.float_format_eqb_eq. solve_eqb_eq.
+Qed. 
+
+Definition ty_eqb_eq := proj1 ty_eqb_eq_aux.
+Definition ty_node_eqb_eq := proj1 (proj2 ty_eqb_eq_aux).
+Definition tysymbol_eqb_eq := proj2 (proj2 ty_eqb_eq_aux).
+
+Definition tysymbol_eq : base.EqDecision tysymbol_c :=
+  dec_from_eqb _ tysymbol_eqb_eq.
+
+
+Module TsymTagged <: TaggedType.
+Definition t := tysymbol_c.
+Definition tag (ts: tysymbol_c) := (ident_of_tysym ts).(id_tag).
+Definition eq := tysymbol_eq.
+End TsymTagged.
+
+Module Tsym := MakeMSH TsymTagged.
+Module Sts := Tsym.S.
+Module Mts := Tsym.M.
+(*Module Hts := Tsym.H
+  Module Wts := Tsym.W*)
+
+Definition ts_equal (t1 t2: tysymbol_c) : bool := tysymbol_eqb t1 t2.
+Definition ty_equal (t1 t2: ty_c) : bool := ty_eqb t1 t2.
+
+Definition ts_hash (ts: tysymbol_c) := id_hash (ident_of_tysym ts).
+Definition ty_hash (t: ty_c) := tag_of_ty t.
+(*For now, skip ts_compare and ty_compare*)
+
+(*Skip Hsty = HashCons.Make...*)
+
+(*TODO: figure out how to extract this*)
+(*Definition mk_ts (name: preid) (args: list tvsymbol) (d: type_def_c) : 
+  ctr tysymbol_c :=
+  ctr_bnd (fun i => ctr_ret (mk_ts_c i args d)) (id_register name).*)
+
+Definition ty_eq : base.EqDecision ty_c :=
+  dec_from_eqb _ ty_eqb_eq.
+
+Module TyTagged <: TaggedType.
+Definition t := ty_c.
+Definition tag (t: ty_c) := tag_of_ty t.
+Definition eq := ty_eq.
+End TyTagged.
+
+Module TyM := MakeMSH TyTagged.
+Module Sty := TyM.S.
+Module Mty := TyM.M.
+(*Module Hty := Ty.H
+  Module Wty := Ty.W*)
