src/util/Number.v
@@ -1,4 +1,5 @@
 (*Why3 Number uses BigInt; we will use Z*)
+Require Import CoqUtil.
 Require CoqBigInt.
 
 (** Range checks *)
@@ -8,8 +9,16 @@ Record int_range := {
 }.
 
 Definition int_range_eqb (i1 i2: int_range) : bool :=
-  CoqBigInt.eq i1.(ir_lower) i2.(ir_lower) &&
-  CoqBigInt.eq i1.(ir_upper) i2.(ir_upper).
+  CoqBigInt.eqb i1.(ir_lower) i2.(ir_lower) &&
+  CoqBigInt.eqb i1.(ir_upper) i2.(ir_upper).
+
+Lemma int_range_eqb_eq i1 i2: i1 = i2 <-> int_range_eqb i1 i2.
+Proof.
+  destruct i1 as [l1 u1]; destruct i2 as [l2 u2]; 
+  unfold int_range_eqb; simpl.
+  rewrite andb_true, <- !CoqBigInt.eqb_eq.
+  solve_eqb_eq.
+Qed.
 
 Definition create_range lo hi : int_range :=
   {| ir_lower := lo; ir_upper := hi|}.
@@ -20,5 +29,13 @@ Record float_format := {
 }.
 
 Definition float_format_eqb (i1 i2: float_format) : bool :=
-  CoqBigInt.eq i1.(fp_exponent_digits) i2.(fp_exponent_digits) &&
-  CoqBigInt.eq i1.(fp_significand_digits) i2.(fp_significand_digits).
+  CoqBigInt.eqb i1.(fp_exponent_digits) i2.(fp_exponent_digits) &&
+  CoqBigInt.eqb i1.(fp_significand_digits) i2.(fp_significand_digits).
+
+Lemma float_format_eqb_eq i1 i2: i1 = i2 <-> float_format_eqb i1 i2.
+Proof.
+  destruct i1 as [e1 s1]; destruct i2 as [e2 s2]; 
+  unfold float_format_eqb; simpl.
+  rewrite andb_true, <- !CoqBigInt.eqb_eq.
+  solve_eqb_eq.
+Qed.
